Prove redc property

montgomery-correctness.ec
@@ -3,18 +3,123 @@ require import Montgomery.
 from Jasmin require import JModel.
 
 op dilithium_modulo = 8380417.
+op dilithium_modulo_left_shift41 = 18428731874223325184.
+op dilithium_modulo_inv = 58728449.
 
-module Correctness = {
-	proc brute_force_mod_check(v: int) : bool = {
-		var correct_answer : W64.t;
-		var computed_answer : W64.t;
+(*
+lemma dilithium_mod_right_inv_correct:
+    dilithium_modulo * dilithium_modulo_inv %% (2 ^ 32) = 1.
+proof.
+    trivial.
+qed.
 
-		computed_answer <@ M.brute_force_mod(W64.of_int v);
-		correct_answer <- W64.of_int (v %% dilithium_modulo);
-		return (computed_answer = correct_answer);
-	}
-}.
+lemma dilithium_mod_left_inv_correct:
+    dilithium_modulo_inv * dilithium_modulo %% (2 ^ 32) = 1.
+proof.
+    trivial.
+qed.
+  *)
 
-(* Check somewhere that v is int64? *)
+lemma dilithium_mod_inv_correct:
+    dilithium_modulo_inv * dilithium_modulo %% (2 ^ 32) = 1.
+proof.
+    trivial.
+qed.
+  
+  
+op montgomery = fun (x : int) => (2 ^ 32 * x) %% dilithium_modulo.
 
-(* local lemma brute_force_mod_correctness *)
+op montgomery_redc_m = fun (a' : int) => (-a' * dilithium_modulo_inv) %% (2 ^ 32).
+
+op montgomery_redc_t = fun (a' : int) =>
+    let m = montgomery_redc_m(a') in
+    (a' + m * dilithium_modulo) %/ (2 ^ 32).
+
+op montgomery_redc = fun (a' : int) => 
+    let m = montgomery_redc_m(a') in
+    let t = montgomery_redc_t(a') in
+    if t < dilithium_modulo then t else t - dilithium_modulo.
+
+lemma montgomery_correct_div_t:
+    forall a', 0 <= a' < dilithium_modulo =>
+    montgomery_redc_t(a') * (2 ^ 32) = a' + montgomery_redc_m(a') * dilithium_modulo.
+proof.
+    move => a' a'_range.
+    have r_divides_mN: (a' + montgomery_redc_m(a') * dilithium_modulo) %% 2 ^ 32 = 0.
+        rewrite /montgomery_redc_m.
+        rewrite - modzDmr.
+        rewrite modzMml.
+
+        have move_a':
+            (- a' * dilithium_modulo_inv) * dilithium_modulo =
+            dilithium_modulo_inv * dilithium_modulo * (-a').
+            (* I really didn't want to hit associativity with smt... *)
+            smt.
+        rewrite move_a'.
+        rewrite - modzMml .
+        rewrite dilithium_mod_inv_correct.
+        apply modzDmr.
+    rewrite /montgomery_redc_t.
+    simplify.
+    rewrite divzE.
+    rewrite r_divides_mN.
+    simplify.
+done.
+
+(*
+251 (* -------------------------------------------------------------------- *)
+252 lemma nosmt modzE m d : m %% d = m - (m %/ d) * d.
+253 proof. by have [+ _] - {2}-> := edivzP m d; rewrite addrAC addrN. qed.
+254
+255 (* -------------------------------------------------------------------- *)
+256 lemma nosmt divzE m d : m %/ d * d = m - m %% d.
+257 proof. by rewrite modzE; ring. qed.
+*)
+    
+
+    
+            
+    
+
+
+
+        
+
+
+
+
+
+(* Add-linear?
+Want: (a%d + b%d) %d = (a+b)%d
+*)
+
+(*
+337 lemma nosmt modzDml m n d : (m %% d + n) %% d = (m + n) %% d.
+338 proof. by rewrite {2}(divz_eq m d) -addrA modzMDl. qed.
+339
+340 lemma nosmt modzDmr m n d : (m + n %% d) %% d = (m + n) %% d.
+341 proof. by rewrite !(addrC m) modzDml. qed.
+*)
+
+(* mult-linear: modzMml *)
+(* modzMml m n d : ((m %% d) * n) %% d = (m * n) %% d *)
+    
+
+    
+    
+
+
+
+    
+
+
+lemma montgomery_redc_is_left_inv:
+    forall x, 0 <= x < 2 ^ 32 => montgomery_redc(montgomery(x)) = x.
+proof.
+    move => x x_range.
+    
+
+
+
+
+
